zero_or_more Pulse skeleton

src/cddl/pulse/CDDL.Pulse.Serialize.Gen.MapGroup.ZeroOrMore.Aux2.fst
@@ -1,5 +1,11 @@
 module CDDL.Pulse.Serialize.Gen.MapGroup.ZeroOrMore.Aux2
 #lang-pulse
+open CDDL.Pulse.Serialize.Gen.MapGroup.ZeroOrMore.Aux2.Proof0
+
+module GR = Pulse.Lib.GhostReference
+module S = Pulse.Lib.Slice
+
+#push-options "--z3rlimit 64"
 
 inline_for_extraction noextract [@@noextract_to "krml"]
 fn impl_serialize_map_zero_or_more_iterator_gen
@@ -38,5 +44,129 @@ fn impl_serialize_map_zero_or_more_iterator_gen
     (out_size: _)
     (l: _)
 {
-  admit ()
+  let mut pres = true;
+  let mut pc = c0;
+  let em0 = is_empty _ _ c0;
+  let mut pem = em0;
+  Trade.refl (r _ _ c0 v0);
+  S.pts_to_len out;
+  let gm = GR.alloc (Ghost.reveal l);
+  with size0 . assert (pts_to out_size size0);
+  with w0 . assert (pts_to out w0);
+  with count0 . assert (pts_to out_count count0);
+  assert pure (cbor_parse_map_prefix_prop' p (U64.v count0) w0 (Seq.slice w0 0 (SZ.v size0)));
+  assume pure (
+    impl_serialize_map_zero_or_more_iterator_gen_invariant p em0 out w0 size0 count0 l v0 true
+  );
+  while (
+    !pres && not !pem
+  )
+  invariant exists* c v em res vout size count m .
+    pts_to out vout **
+    pts_to pc c **
+    r _ _ c v **
+    Trade.trade (r _ _ c v) (r _ _ c0 v0) **
+    pts_to pem em **
+    pts_to pres res **
+    GR.pts_to gm m **
+    pts_to out_size size **
+    pts_to out_count count **
+    pure (
+      impl_serialize_map_zero_or_more_iterator_gen_invariant p em out vout size count m v res
+    )
+  {
+    let count = !out_count;
+    if (count = pow2_64_m1) {
+      pres := false;
+      assume pure False
+    } else {
+      let count' = U64.add count 1uL;
+      S.pts_to_len out;
+      with w0 . assert (pts_to out w0);
+      let (ek, ev) = next _ _ pc;
+      Trade.trans _ _ (r _ _ c0 v0);
+      with gk . assert (dsnd (Iterator.mk_spec r1) (fst (ek, ev)) gk);
+      Trade.rewrite_with_trade
+        (dsnd (Iterator.mk_spec r1) (fst (ek, ev)) gk)
+        (r1 ek gk);
+      let size0 = !out_size;
+      let (_, out1) = slice_split out size0;
+      let size1 = pa1 ek out1;
+      S.pts_to_len out1;
+      Trade.elim (r1 ek gk) _;
+      if (size1 = 0sz) {
+        Pulse.Lib.Slice.join _ _ _;
+        Trade.elim_hyp_l _ _ _;
+        pres := false;
+        assume pure False
+      } else {
+        let (out1', out2) = slice_split out1 size1;
+        with gv . assert (dsnd (Iterator.mk_spec r2) (snd (ek, ev)) gv);
+        Trade.rewrite_with_trade
+          (dsnd (Iterator.mk_spec r2) (snd (ek, ev)) gv)
+          (r2 ev gv);
+        let size2 = pa2 ev out2;
+        S.pts_to_len out2;
+        Trade.elim (r2 ev gv) _;
+        Trade.elim_hyp_l _ _ _;
+        if (size2 = 0sz) {
+          Pulse.Lib.Slice.join _ _ out1;
+          Pulse.Lib.Slice.join _ _ _;
+          pres := false;
+          assume pure False
+        } else {
+          let ock = parse out1';
+          assert pure (Some? ock);
+          let Some ck_ = ock;
+          let (ck, remk) = ck_;
+          with wk . assert (cbor_parse_post pe vmatch' out1' 1.0R wk (Some (ck, remk)));
+          rewrite (cbor_parse_post pe vmatch' out1' 1.0R wk (Some (ck, remk)))
+            as (cbor_parse_post_some pe vmatch' out1' 1.0R wk ck remk);
+          unfold (cbor_parse_post_some pe vmatch' out1' 1.0R wk ck remk);
+          with vk . assert (vmatch' 1.0R ck vk);
+          let (out2', _) = slice_split out2 size2;
+          let ocv = parse out2';
+          assert pure (Some? ocv);
+          let Some cv_ = ocv;
+          let (cv, remv) = cv_;
+          with wv . assert (cbor_parse_post pe vmatch' out2' 1.0R wv (Some (cv, remv)));
+          rewrite (cbor_parse_post pe vmatch' out2' 1.0R wv (Some (cv, remv)))
+            as (cbor_parse_post_some pe vmatch' out2' 1.0R wv cv remv);
+          unfold (cbor_parse_post_some pe vmatch' out2' 1.0R wv cv remv);
+          with vv . assert (vmatch' 1.0R cv vv);
+          let ce = mk_map_entry ck cv;
+          let ex = va_ex ce;
+          Trade.elim (vmatch2' 1.0R ce _) _;
+          Trade.elim (vmatch' 1.0R ck _ ** _) _;
+          Trade.elim (vmatch' 1.0R cv _ ** _) _;
+          Pulse.Lib.Slice.join _ _ out2;
+          Pulse.Lib.Slice.join _ _ out1;
+          Pulse.Lib.Slice.join _ _ _;
+          S.pts_to_len out;
+          if (ex) {
+            pres := false;
+            assume pure False
+          } else {
+            let size1' = SZ.add size0 size1;
+            let size2' = SZ.add size1' size2;
+            let (out_, _) = slice_split out size2';
+            with w_ . assert (pts_to out_ w_);
+            with m . assert (GR.pts_to gm m);
+            assume pure (cbor_serialize_map_insert_pre p pe m size0 vk size1' vv w_);
+            let no_dup = insert out_ m size0 vk size1' vv;
+            Pulse.Lib.Slice.join _ _ _;
+            S.pts_to_len out;
+            pem := is_empty _ _ !pc;
+            out_size := size2';
+            out_count := count';
+            assume pure False
+          }
+        }
+      }
+    }
+  };
+  Trade.elim _ _;
+  GR.free gm;
+  assume pure False;
+  !pres
 }
