src/cddl/pulse/CDDL.Pulse.Serialize.Gen.MapGroup.ZeroOrMore.Aux2.Invariant.fst
@@ -1,0 +1,71 @@
+module CDDL.Pulse.Serialize.Gen.MapGroup.ZeroOrMore.Aux2.Invariant
+include CDDL.Pulse.Serialize.Gen.MapGroup.ZeroOrMore.Aux1
+
+module Trade = Pulse.Lib.Trade.Util
+module R = Pulse.Lib.Reference
+module S = Pulse.Lib.Slice
+module U8 = FStar.UInt8
+module SZ = FStar.SizeT
+module Cbor = CBOR.Spec.API.Format
+module U64 = FStar.UInt64
+module Iterator = CDDL.Pulse.Iterator.Base
+module EqTest = CDDL.Spec.EqTest
+
+module GR = Pulse.Lib.GhostReference
+module Map = CDDL.Spec.Map
+
+module SM = Pulse.Lib.SeqMatch
+
+inline_for_extraction noextract [@@noextract_to "krml";
+  FStar.Tactics.postprocess_with (fun _ -> FStar.Tactics.norm [delta; zeta; iota; primops]; FStar.Tactics.trefl ())
+]
+let pow2_64_m1 : U64.t = U64.uint_to_t (pow2 64 - 1)
+
+let pow2_64_m1_eq : squash (U64.v pow2_64_m1 == pow2 64 - 1) = _ by (
+  FStar.Tactics.norm [delta; zeta; iota; primops];
+  FStar.Tactics.trefl ()
+)
+
+let impl_serialize_map_zero_or_more_iterator_gen_invariant0
+  (#pe: cbor_parser)
+  (#minl: (cbor_min_length pe))
+  (#maxl: (cbor_max_length pe))
+  (#tkey: Type)
+  (#tvalue: Type)
+  (p: (cbor_map_parser minl maxl))
+  (em: bool)
+  (out: S.slice U8.t)
+  (vout: Seq.seq U8.t)
+  (size: SZ.t)
+  (count: U64.t)
+  (m: cbor_map)
+  (v: Map.t tkey (list tvalue))
+  (res: bool)
+: prop
+=
+      Seq.length vout == SZ.v (S.len out) /\
+      SZ.v size <= Seq.length vout /\
+      (
+        res == true ==> (
+          cbor_map_length m == U64.v count /\
+          p (U64.v count) (Seq.slice vout 0 (SZ.v size)) == Some (m, SZ.v size) /\
+          (em == true <==> v == Map.empty _ _)
+        )
+      )
+
+assume val impl_serialize_map_zero_or_more_iterator_gen_invariant
+  (#pe: cbor_parser)
+  (#minl: (cbor_min_length pe))
+  (#maxl: (cbor_max_length pe))
+  (#tkey: Type)
+  (#tvalue: Type)
+  (p: (cbor_map_parser minl maxl))
+  (em: bool)
+  (out: S.slice U8.t)
+  (vout: Seq.seq U8.t)
+  (size: SZ.t)
+  (count: U64.t)
+  (m: cbor_map)
+  (v: Map.t tkey (list tvalue))
+  (res: bool)
+: prop
