src/cddl/pulse/CDDL.Pulse.Serialize.Gen.MapGroup.ZeroOrMore.Aux2.Proof0.fsti
@@ -1,0 +1,37 @@
+module CDDL.Pulse.Serialize.Gen.MapGroup.ZeroOrMore.Aux2.Proof0
+include CDDL.Pulse.Serialize.Gen.MapGroup.ZeroOrMore.Aux2.Invariant
+
+module Trade = Pulse.Lib.Trade.Util
+module R = Pulse.Lib.Reference
+module S = Pulse.Lib.Slice
+module U8 = FStar.UInt8
+module SZ = FStar.SizeT
+module Cbor = CBOR.Spec.API.Format
+module U64 = FStar.UInt64
+module Iterator = CDDL.Pulse.Iterator.Base
+module EqTest = CDDL.Spec.EqTest
+
+module GR = Pulse.Lib.GhostReference
+module Map = CDDL.Spec.Map
+
+module SM = Pulse.Lib.SeqMatch
+
+val impl_serialize_map_zero_or_more_iterator_gen_invariant_implies_invariant0
+  (#pe: cbor_parser)
+  (#minl: (cbor_min_length pe))
+  (#maxl: (cbor_max_length pe))
+  (#tkey: Type)
+  (#tvalue: Type)
+  (p: (cbor_map_parser minl maxl))
+  (em: bool)
+  (out: S.slice U8.t)
+  (vout: Seq.seq U8.t)
+  (size: SZ.t)
+  (count: U64.t)
+  (m: cbor_map)
+  (v: Map.t tkey (list tvalue))
+  (res: bool)
+: Lemma
+  (requires impl_serialize_map_zero_or_more_iterator_gen_invariant p em out vout size count m v res)
+  (ensures impl_serialize_map_zero_or_more_iterator_gen_invariant0 p em out vout size count m v res)
+  [SMTPat (impl_serialize_map_zero_or_more_iterator_gen_invariant p em out vout size count m v res)]
